# 微分形式计算题详细解释

## 问题(1)的详细步骤：
$(x\mathrm{d}x+7z^{2}\mathrm{d}y)\wedge(y\mathrm{d}x-x\mathrm{d}y+6\mathrm{d}z)$

**展开过程：**
- $x\mathrm{d}x \wedge y\mathrm{d}x = xy(\mathrm{d}x \wedge \mathrm{d}x) = 0$ （因为 $\mathrm{d}x \wedge \mathrm{d}x = 0$）
- $x\mathrm{d}x \wedge (-x\mathrm{d}y) = -x^2(\mathrm{d}x \wedge \mathrm{d}y)$
- $x\mathrm{d}x \wedge 6\mathrm{d}z = 6x(\mathrm{d}x \wedge \mathrm{d}z)$
- $7z^{2}\mathrm{d}y \wedge y\mathrm{d}x = 7yz^{2}(\mathrm{d}y \wedge \mathrm{d}x) = -7yz^{2}(\mathrm{d}x \wedge \mathrm{d}y)$
- $7z^{2}\mathrm{d}y \wedge (-x\mathrm{d}y) = -7xz^{2}(\mathrm{d}y \wedge \mathrm{d}y) = 0$
- $7z^{2}\mathrm{d}y \wedge 6\mathrm{d}z = 42z^{2}(\mathrm{d}y \wedge \mathrm{d}z)$

**合并整理：**
$-x^2(\mathrm{d}x \wedge \mathrm{d}y) - 7yz^{2}(\mathrm{d}x \wedge \mathrm{d}y) + 6x(\mathrm{d}x \wedge \mathrm{d}z) + 42z^{2}(\mathrm{d}y \wedge \mathrm{d}z)$

**利用反称性：**
$\mathrm{d}x \wedge \mathrm{d}z = -\mathrm{d}z \wedge \mathrm{d}x$

**最终结果：**
$-\left(x^{2}+7yz^{2}\right)\mathrm{d}x\wedge\mathrm{d}y+42z^{2}\mathrm{d}y\wedge\mathrm{d}z-6x\mathrm{d}z\wedge\mathrm{d}x$

## 问题(2)的详细步骤：
$(\cos y\mathrm{d}x+\cos x\mathrm{d}y)\wedge(\sin y\mathrm{d}x-\sin x\mathrm{d}y)$

**展开过程：**
- $\cos y\mathrm{d}x \wedge \sin y\mathrm{d}x = \cos y\sin y(\mathrm{d}x \wedge \mathrm{d}x) = 0$
- $\cos y\mathrm{d}x \wedge (-\sin x\mathrm{d}y) = -\cos y\sin x(\mathrm{d}x \wedge \mathrm{d}y)$
- $\cos x\mathrm{d}y \wedge \sin y\mathrm{d}x = \cos x\sin y(\mathrm{d}y \wedge \mathrm{d}x) = -\cos x\sin y(\mathrm{d}x \wedge \mathrm{d}y)$
- $\cos x\mathrm{d}y \wedge (-\sin x\mathrm{d}y) = -\cos x\sin x(\mathrm{d}y \wedge \mathrm{d}y) = 0$

**合并整理：**
$-\cos y\sin x(\mathrm{d}x \wedge \mathrm{d}y) - \cos x\sin y(\mathrm{d}x \wedge \mathrm{d}y)$
$= -(\cos y\sin x + \cos x\sin y)(\mathrm{d}x \wedge \mathrm{d}y)$

**利用三角恒等式：**
$\cos y\sin x + \cos x\sin y = \sin(x+y)$

**最终结果：**
$-\sin(x+y)\mathrm{d}x\wedge\mathrm{d}y$

## 问题(3)的详细步骤：
$(6\mathrm{d}x\wedge\mathrm{d}y+27\mathrm{d}x\wedge\mathrm{d}z)\wedge(\mathrm{d}x+\mathrm{d}y+\mathrm{d}z)$

**展开过程：**
- $6\mathrm{d}x\wedge\mathrm{d}y \wedge \mathrm{d}x = 6(\mathrm{d}x\wedge\mathrm{d}y\wedge\mathrm{d}x) = 0$ （因为 $\mathrm{d}x$ 重复）
- $6\mathrm{d}x\wedge\mathrm{d}y \wedge \mathrm{d}y = 6(\mathrm{d}x\wedge\mathrm{d}y\wedge\mathrm{d}y) = 0$ （因为 $\mathrm{d}y$ 重复）
- $6\mathrm{d}x\wedge\mathrm{d}y \wedge \mathrm{d}z = 6(\mathrm{d}x\wedge\mathrm{d}y\wedge\mathrm{d}z)$
- $27\mathrm{d}x\wedge\mathrm{d}z \wedge \mathrm{d}x = 27(\mathrm{d}x\wedge\mathrm{d}z\wedge\mathrm{d}x) = 0$ （因为 $\mathrm{d}x$ 重复）
- $27\mathrm{d}x\wedge\mathrm{d}z \wedge \mathrm{d}y = 27(\mathrm{d}x\wedge\mathrm{d}z\wedge\mathrm{d}y) = -27(\mathrm{d}x\wedge\mathrm{d}y\wedge\mathrm{d}z)$
- $27\mathrm{d}x\wedge\mathrm{d}z \wedge \mathrm{d}z = 27(\mathrm{d}x\wedge\mathrm{d}z\wedge\mathrm{d}z) = 0$ （因为 $\mathrm{d}z$ 重复）

**合并整理：**
$6(\mathrm{d}x\wedge\mathrm{d}y\wedge\mathrm{d}z) - 27(\mathrm{d}x\wedge\mathrm{d}y\wedge\mathrm{d}z) = -21\mathrm{d}x\wedge\mathrm{d}y\wedge\mathrm{d}z$

**最终结果：**
$-21\mathrm{d}x\wedge\mathrm{d}y\wedge\mathrm{d}z$
